theories/Compositional_Structures/Basic_Modules/Plurality_Module_Ref.thy
@@ -1,229 +1,60 @@
 theory Plurality_Module_Ref
-  imports 
-        "Verified_Voting_Rule_Construction.Plurality_Module"
-        "Component_Types/Social_Choice_Types/Profile_List_Monadic"
-        "Component_Types/Electoral_Module_Ref"
-    
+  imports "Verified_Voting_Rule_Construction.Plurality_Module"
+           "Component_Types/Elimination_Module_Ref"
 begin
 
 
-definition compute_scores :: "'a set \<Rightarrow> 'a Profile_List \<Rightarrow> ('a \<rightharpoonup> nat) nres" 
-  where "compute_scores A p \<equiv>
-  FOREACH A 
-    (\<lambda>x m. do {
-      scx \<leftarrow> (wc_fold p x);
-      RETURN (m(x\<mapsto>scx))
-  }) (Map.empty)"
+fun plur_score_mon :: "'a Evaluation_Function_Ref" where
+  "plur_score_mon x A p = (wc_fold p x)"
 
-
-definition "scoremax A scores \<equiv> do {
-  FOREACH (A)
-    (\<lambda>x max. do {
-      ASSERT (x \<in> dom scores);
-      let scx = the (scores x);
-      (if (scx > max) then 
-          RETURN (scx) 
-      else 
-          RETURN(max))
-    }) (0::nat)
+definition plarility_monadic :: "'a Electoral_Module_Ref" where
+  "plarility_monadic A pl \<equiv> do {
+   scores <- (pre_compute_scores plur_score_mon A pl);
+   max_eliminator_ref scores A pl
 }"
-
-definition pluralityparam ::
-    "'a set \<Rightarrow> ('a \<Rightarrow> nat option) \<Rightarrow> nat \<Rightarrow> 'a Result nres" where 
-"pluralityparam A scores threshold \<equiv>
-    FOREACH (A)
-    (\<lambda>x (e,r,d). do {
-      ASSERT (x \<in> dom scores);
-      let scx = the (scores x);
-      let sel = threshold;
-      (if (scx = sel) then 
-          RETURN (insert x e,r,d) 
-      else 
-          RETURN(e, insert x r,d))
-    }) ({},{},{})"
-
-(* TODO: think about creating a locale like Kruskal AFP 
-  where the precompute map monad can be an assumption *)
-definition plurality_init:: "'a Electoral_Module_Ref" where 
-"plurality_init A p \<equiv> do {
-  scores <- compute_scores A p;
-  threshold <- (scoremax A scores);
-  pluralityparam A scores threshold
-}"
-
-sepref_definition plurality_sepref is
-  "uncurry plurality_init":: 
-    "(hs.assn nat_assn)\<^sup>k *\<^sub>a (list_assn (array_assn nat_assn))\<^sup>k 
-   \<rightarrow>\<^sub>a ((hs.assn nat_assn) \<times>\<^sub>a (hs.assn nat_assn) \<times>\<^sub>a (hs.assn nat_assn))"
-  unfolding plurality_init_def[abs_def] pluralityparam_def[abs_def] 
-    compute_scores_def[abs_def] wc_fold_def[abs_def] scoremax_def[abs_def] short_circuit_conv
-  apply (rewrite in "FOREACH _ _ \<hole>" hm.fold_custom_empty)
-  apply (rewrite in "FOREACH _ _ \<hole>" hs.fold_custom_empty)+
-  apply sepref_dbg_keep
-  done
-
-thm plurality_sepref.refine
-
-export_code plurality_sepref in Scala_imp
 
 context voting_session
 begin
 
-definition "precompute_map \<equiv> (\<lambda>a. Some (win_count pr a))|`A"
+lemma plur_score_refine:
+  shows "plur_score_mon x A pl \<le> SPEC (\<lambda> ps. ps =  plur_score x A pr)"
+proof (unfold plur_score_mon.simps plur_score.simps)
+  from profrel have profl: "profile_l A pl" using profile_prop_list
+    by blast
+  from profrel have prel: "(pl, pr) \<in> profile_rel" 
+    using profile_type_ref by blast
+  from  profl prel wc_fold_correct 
+  show "wc_fold pl x \<le> SPEC (\<lambda>ps. ps = win_count pr x)"
+    by fastforce
+qed
 
-definition "max_comp_plurality \<equiv> Max {win_count pr x |x. x \<in> A}"
-
-lemma plurality_monadic_correct:
-  shows "(pluralityparam A precompute_map max_comp_plurality
-           ,(SPEC (\<lambda> elecres. elecres = plurality A pr))) \<in> \<langle>Id\<rangle>nres_rel "
-  unfolding pluralityparam_def precompute_map_def max_comp_plurality_def
-  apply (refine_vcg FOREACH_rule[where I = 
-        "(\<lambda>it (e,r,d). (\<forall>elem \<in> e.  \<forall>a \<in> A. win_count pr a \<le> win_count pr elem)
-          \<and> (\<forall>elem \<in> r.  \<exists>a \<in> A. win_count pr a > win_count pr elem)
-          \<and> d = {} 
-          \<and> e \<union> r = (A - it))"] )
-  apply (clarsimp_all simp add: fina
-    simp del: win_count.simps )
-  subgoal by auto
-  using fina score_bounded[where A= A and f=win_count]
-  using fina nempa max_score_in[where A= A and f=win_count] 
-  apply (rename_tac e r alt)
-  using leD 
-   (*apply (metis UnCI leD)+*)
-  sorry
-
-
-lemma compute_scores_correct:
-  shows "(compute_scores A pl, SPEC (\<lambda> map. map = precompute_map)) \<in> \<langle>Id\<rangle>nres_rel"
-  unfolding compute_scores_def precompute_map_def
-  apply (refine_vcg FOREACH_rule[where I = 
-        "(\<lambda>it r. r = (\<lambda> e. Some (win_count (pr) e))|`(A - it))"])
-  apply (auto simp add: fina simp del: win_count.simps)
-proof -
-  fix x:: 'a
-  fix it:: "'a set"
-  assume xit: "x \<in> it"
-  assume itA: "it \<subseteq> A"
-  from xit itA have xiA: "x \<in> A" by fastforce
-  from xit itA have wcr: "((\<lambda>e. Some (win_count pr e)) |` (A - it))(x \<mapsto> win_count pr x) =
-                      (\<lambda>e. Some (win_count pr e)) |` (A - (it - {x}))"
-      using it_step_insert_iff restrict_map_insert
-      by metis
-  from this have mapupdeq: "(\<lambda>scx. ((\<lambda>e. Some (win_count pr e)) |` (A - it))(x \<mapsto> scx) =
-                   (\<lambda>e. Some (win_count pr e)) |` (A - (it - {x})))
-      = (\<lambda> wc. wc = win_count pr x)"
-    by (metis map_upd_eqD1)
-  from profrel have prel: "(pl, pr) \<in> profile_rel" using profile_type_ref by auto
-  from profrel have "profile_l A pl" using profile_prop_list by auto 
-  from prel this have "wc_fold pl x \<le> SPEC(\<lambda> scx. scx = win_count pr x)"
-    using wc_fold_correct by auto
-  from this mapupdeq show " wc_fold pl x
-       \<le> SPEC (\<lambda>scx. ((\<lambda>e. Some (win_count pr e)) |` (A - it))(x \<mapsto> scx) =
-                      (\<lambda>e. Some (win_count pr e)) |` (A - (it - {x})))"
-    using SPEC_cons_rule it_step_insert_iff restrict_map_insert
-    by presburger 
-qed 
-
-
-lemma scoremax_correct:
-  shows "(scoremax A precompute_map, SPEC (\<lambda> th. th =  max_comp_plurality)) \<in> \<langle>nat_rel\<rangle>nres_rel"
-  unfolding scoremax_def max_comp_plurality_def precompute_map_def
-  apply (refine_vcg FOREACH_rule[where I = "(\<lambda>it max. (\<forall>a \<in> (A - it). win_count pr a \<le> max) 
-\<and> ((\<exists>e \<in> (A - it). max = win_count pr e) \<or> max = 0))"] )
-  apply (auto simp add: fina simp del: win_count.simps)
-  apply (metis Diff_iff leD nle_le order_trans)
-    apply (metis DiffI order_less_imp_le)
-  using fina score_bounded[where A= A and p = pr and f=win_count]
-  nempa nbexmax[where A= A and p = pr and f=win_count]
-
-  sorry
-  (*apply (metis antisym linorder_not_le max_comp_plurality_def)
-  using fina nempa nbexmax[where A= A and p = pr and f=win_count]
-  apply (simp add: finite_nat_set_iff_bounded)
-  done*)
-
-lemma parameterized_refinement: 
-  "(pluralityparam, pluralityparam) \<in> \<langle>Id\<rangle>set_rel \<rightarrow> Id \<rightarrow> nat_rel \<rightarrow> \<langle>Id\<rangle>nres_rel"
-  unfolding pluralityparam_def
-  apply (refine_vcg)
-  apply (auto simp add: refine_rel_defs)[3]
-  apply clarsimp_all
-  done
-
-
-(*lemma rewritep: "((RETURN precompute_map) \<bind> 
-(\<lambda> map. pluralityparam A map (scoremax A map)), 
-pluralityparam A precompute_map max_comp_plurality)
-  \<in> \<langle>Id\<rangle>nres_rel"
-  apply clarsimp
-  apply refine_vcg
-proof -
-  have refi: "scoremax A precompute_map \<le> \<Down> Id max_comp_spec_plurality"
-    using scoremax_correct nres_relD by blast
-  have "(A,A) \<in> \<langle>Id\<rangle>set_rel"
-    by simp 
-  show "pluralityparam A precompute_map (scoremax A precompute_map)
-    \<le> \<Down> Id (pluralityparam A precompute_map max_comp_spec_plurality)"
-    unfolding pluralityparam_def
-    apply refine_vcg
-    apply (refine_dref_type)
-    apply (auto simp add: refine_rel_defs)
-    using refi refine_IdD by blast
-qed*)
-
-
-(*lemma scores_param: "(compute_scores A pl \<bind> (\<lambda> map. pluralityparam A map 
-  (scoremax A map)), pluralityparam A precompute_map max_comp_plurality)
-  \<in> \<langle>Id\<rangle>nres_rel"
-  using rewritep compute_scores_correct in_nres_rel_iff
-  by (metis (no_types, lifting) BNF_Greatest_Fixpoint.IdD Collect_cong Id_refine 
-SPEC_eq_is_RETURN(2) bind_refine conc_trans_additional(5)) *)
-
-find_theorems bind
-
-lemma plurality_init_refine:
-  shows "(plurality_init A pl, (pluralityparam A precompute_map max_comp_plurality))
-      \<in> \<langle>Id\<rangle>nres_rel"
-  apply (rule nres_relI)
-  apply (simp add: Id_refine)
-  unfolding plurality_init_def
-proof -
-  have "SPEC(\<lambda> map. map =precompute_map) \<bind> (\<lambda>scores. scoremax A scores \<bind> pluralityparam A scores)
-    \<le> pluralityparam A precompute_map max_comp_plurality"
-    using scoremax_correct[THEN nres_relD, THEN refine_IdD]
-    by (metis (no_types, lifting) Collect_cong RETURN_SPEC_conv Refine_Basic.bind_mono(1) let_to_bind_conv order_mono_setup.refl) 
-  from this show "compute_scores A pl \<bind> (\<lambda>scores. scoremax A scores \<bind> pluralityparam A scores)
-    \<le> pluralityparam A precompute_map max_comp_plurality"
-    using compute_scores_correct[THEN nres_relD, THEN refine_IdD]
-    using Refine_Basic.bind_mono(1) dual_order.trans by blast
-qed 
-  
-
-(*lemmas plurality_init_refspec = plurality_init_refine[FCOMP plurality_monadic_correct]*)
-
-theorem plurality_init_correct:
-  shows "(plurality_init A pl, (SPEC (\<lambda> elecres. elecres = plurality A pr)))
-     \<in> \<langle>Id\<rangle>nres_rel"
-  apply (rule nres_relI)
-  apply (rule refine_IdI)
-  using plurality_monadic_correct[THEN nres_relD, THEN refine_IdD]
-  using ref_two_step[OF plurality_init_refine[THEN nres_relD] 
-plurality_monadic_correct[THEN nres_relD, THEN refine_IdD], THEN refine_IdD]
-  by fastforce
-  
-
-theorem plurality_init_dataref:
-  shows "(plurality_init, (\<lambda> Alts p. SPEC (\<lambda> elec. elec = (plurality) Alts p)))
-     \<in> \<langle>Id\<rangle>set_rel \<rightarrow> (profile_rel) \<rightarrow> \<langle>Id\<rangle>nres_rel"
+lemma plurality_elim_correct:
+  shows "plarility_monadic A pl \<le> SPEC (\<lambda> res. res = plurality_mod A pr)"
+  unfolding plarility_monadic_def max_eliminator_ref.simps less_eliminator_ref.simps  
+  elimination_module_ref_def eliminate_def
+proof (refine_vcg, unfold plurality_mod.simps)
 
   oops
-
-(*lemmas pluralitysep_correct= "plurality_sepref.refine[FCOMP plurality_init_dataref]"*)
 
 end
 
 
+sepref_definition plurality_elim_sepref is
+  "uncurry plarility_monadic":: 
+    "(hs.assn nat_assn)\<^sup>k *\<^sub>a (list_assn (array_assn nat_assn))\<^sup>k 
+   \<rightarrow>\<^sub>a ((hs.assn nat_assn) \<times>\<^sub>a (hs.assn nat_assn) \<times>\<^sub>a (hs.assn nat_assn))"
+  unfolding plarility_monadic_def  max_eliminator_ref.simps plur_score_mon.simps
+    less_eliminator_ref.simps  elimination_module_ref_def[abs_def] eliminate_def[abs_def]
+    pre_compute_scores_def[abs_def] scoremax_def[abs_def] wc_fold_def[abs_def] short_circuit_conv
+  apply (rewrite in "FOREACH _ _ \<hole>" hm.fold_custom_empty)
+  apply (rewrite in "FOREACH _ _ \<hole>" hs.fold_custom_empty)
+  apply (rewrite in "FOREACH _ _ \<hole>" hs.fold_custom_empty)
+  apply (rewrite in "_ \<bind> (\<lambda>(rej, def). if def = {} then RETURN (\<hole>, _, rej) else RETURN ({}, rej, def))" hs.fold_custom_empty)
+  apply (rewrite in "_ \<bind> (\<lambda>(rej, def). if def = {} then RETURN (_, \<hole>, rej) else RETURN ({}, rej, def))" hs.fold_custom_empty)
+  apply (rewrite in "_ \<bind> (\<lambda>(rej, def). if def = {} then RETURN (_, _, rej) else RETURN (\<hole>, rej, def))" hs.fold_custom_empty)
 
-  
+  apply sepref_dbg_keep
+  done
+
 
 end
